src/SepExpr.v
@@ -195,10 +195,14 @@ Module SepExpr (B : Heap).
        ; other := nil
        |}.
 
+    Definition starred u v (T : Type) (F : T -> sexpr fs sfuncs u v) (ls : list T)
+      : sexpr fs sfuncs u v :=
+      fold_right (fun x a => Star (F x) a) Emp ls.
+
     Definition denote uvars vars (h : SHeap uvars vars) :  sexpr fs sfuncs uvars vars :=
       let a := dmap_fold (fun a x y => fold_left (fun a y => Star (Func x y) a) y a) Emp (funcs h) in
-      let c := fold_right (fun x a => Star (Inj x) a) Emp (pures h) in
-      let e := fold_right (fun x a => Star (Const x) a) Emp (other h) in
+      let c := starred (fun x => Inj x) (pures h) in
+      let e := starred (fun x => Const x) (other h) in
       Star a (Star c e).
 
     Definition liftFunctions uvars vars' ext vars
@@ -349,6 +353,13 @@ refine (
         clear. unfold heq. intros. simpl. eapply ST.heq_star_frame; eauto.
       Qed.
 
+      Lemma heq_star_emp : forall a c A C (P Q : sexpr fs sfuncs a c), 
+        heq A A C cs P Q -> 
+        heq A A C cs (Star Emp P) Q.
+      Proof.
+        clear. unfold heq. intros. simpl. eapply ST.heq_star_emp; eauto.
+      Qed.
+
       Lemma heq_ex : forall t a b A B C (P Q : sexpr fs sfuncs a (t :: b)), 
         (forall v, heq A B (HCons v C) cs P Q) ->
         heq A B C cs (Exists t P) (Exists t Q).
@@ -466,8 +477,8 @@ refine (
            generalize E f h. uip_all. clear.
              simpl. destruct (get sfuncs f0); simpl in *.
             generalize dependent SDomain0. induction SDomain0.
-            intros. rewrite (hlist_nil_only h0). simpl. eapply ST.Refl_heq.
-            intros. rewrite (hlist_eta h0) in *. simpl in *.
+            intros. rewrite (hlist_nil_only _ h0). simpl. eapply ST.Refl_heq.
+            intros. rewrite (hlist_eta _ h0) in *. simpl in *.
             specialize (IHSDomain0 (SDenotation0 (exprD U (hlist_app G G'') (hlist_hd h0))) (hlist_tl h0)).
             generalize (liftExpr_denote (hlist_hd h0) U G G' G'').
             unfold tvar in *. intros. rewrite H. auto.
@@ -539,22 +550,47 @@ refine (
             eapply ST.heq_ex. intros. eapply ST.heq_star_frame; try reflexivity.
             clear. destruct (get sfuncs f); simpl in *.
             generalize dependent SDomain0. induction SDomain0.
-            intros. rewrite (hlist_nil_only h). simpl. eapply ST.Refl_heq.
-            intros. rewrite (hlist_eta h) in *. simpl in *.
+            intros. rewrite (hlist_nil_only _ h). simpl. eapply ST.Refl_heq.
+            intros. rewrite (hlist_eta _ h) in *. simpl in *.
             specialize (IHSDomain0 (SDenotation0 (exprD A C (hlist_hd h))) (hlist_tl h)).
             generalize (@liftExpr_denote _ _ _ nil (t :: nil) vars a (hlist_hd h) A HNil (HCons v HNil) C).
             simpl. intro. unfold tvar in *. rewrite H. auto.
       Qed.
 
-      Lemma lift_lift_app : forall uvars x y z a A C
+      Lemma liftSExpr_liftSExpr_app : forall uvars x y z a
         (P : sexpr fs sfuncs uvars (x ++ z)),
-        heq A A C cs (liftSExpr x y (a ++ z) (liftSExpr x a z P))
-                     (match app_ass _ _ _ in _ = t return sexpr _ _ _ (x ++ t) with
-                        | refl_equal => liftSExpr x (y ++ a) z P
-                      end).
+        (liftSExpr x y (a ++ z) (liftSExpr x a z P)) = 
+        (match app_ass _ _ _ in _ = t return sexpr _ _ _ (x ++ t) with
+           | refl_equal => liftSExpr x (y ++ a) z P
+         end).
       Proof.
-        clear. 
-      Admitted.
+        clear. intros. uip_all.
+        assert (forall e' (P : sexpr fs sfuncs uvars e') (E : e' = x ++ z),
+          liftSExpr x y (a ++ z) (liftSExpr x a z match E in _ = t return sexpr _ _ _ t with
+                                                    | refl_equal => P
+                                                  end) =
+          match e in _ = t return sexpr _ _ _ (x ++ t) with
+            | refl_equal => liftSExpr x (y ++ a) z match E in _ = t return sexpr _ _ _ t with
+                                                     | refl_equal => P
+                                                   end
+          end).
+        clear. do 2 intro. generalize dependent x. generalize dependent y.
+        induction P; intros; simpl; uip_all; subst.
+          generalize e. simpl. uip_all. reflexivity.
+          simpl. rewrite liftExpr_liftExpr_app. uip_all. generalize e0 e1.
+          rewrite <- e1. uip_all. reflexivity.
+          simpl. specialize (IHP1 _ e _ refl_equal). specialize (IHP2 _ e _ refl_equal).
+          simpl in *. rewrite IHP1. rewrite IHP2. clear. generalize e. rewrite <- e. uip_all.
+          reflexivity.
+          subst. specialize (IHP _ e (t :: x) refl_equal). simpl in *.
+          rewrite IHP. clear. generalize e. rewrite <- e. uip_all. reflexivity.
+
+          simpl. rewrite liftExpr_liftExpr_apps. uip_all. generalize e e0. rewrite <- e.
+          uip_all. reflexivity.
+
+          simpl. generalize e; uip_all. reflexivity.
+          eapply (H _ P refl_equal).
+      Qed.
 
       Lemma lift_existsEach_star : forall uvars x z A C
         (P : sexpr fs sfuncs uvars (x ++ z)) Q,
@@ -568,48 +604,86 @@ refine (
           eapply existsEach_heq. intros.
           simpl in *.
           etransitivity. eapply lift_exists_star. eapply heq_ex. intros.
-          eapply heq_star_frame. reflexivity.
-          etransitivity. 
-          eapply (lift_lift_app nil (a :: nil) z x A (HCons v (hlist_app Z C)) Q) .
-          uip_all; simpl in *. uip_all. reflexivity.
+          eapply heq_star_frame. reflexivity. rewrite liftSExpr_liftSExpr_app.
+          uip_all. simpl in *. generalize e. uip_all. reflexivity.
       Qed.
 
-      Lemma lift_existsEach_existsEach_star : forall uvars x y z A C cs (P : sexpr fs sfuncs uvars (x ++ z))  Q,
+      Lemma liftSExpr_existsEach : forall uvars x y z (P : sexpr fs sfuncs uvars _),
+        liftSExpr nil x z (existsEach y z P) = 
+        existsEach y (x ++ z) (liftSExpr y x z P).
+      Proof.
+        induction y; simpl; auto.
+          intros. rewrite IHy. f_equal.
+      Qed.
+
+      Lemma lift_existsEach_existsEach_star : forall uvars x y z A C (P : sexpr fs sfuncs uvars (x ++ z))  Q,
         heq A A C cs (Star (existsEach x z P) (existsEach y z Q))
         (existsEach x _ (existsEach y _ (Star (liftSExpr nil y (x ++ z) P) (liftSExpr y x z Q)))).
       Proof.
         clear. intros.
           etransitivity. eapply lift_existsEach_star. eapply existsEach_heq.
-          intros. unfold heq; simpl.
-          generalize Q P; clear. induction y using rev_ind. admit.
-            intros; simpl in *. repeat rewrite existsEach_peel_back. uip_all.
-            generalize IHy. clear IHy. generalize (hlist_app Z C).
-            simpl in *. intros. eapply ST.heq_star_comm. 
-            etransitivity. eapply ST.heq_ex_star. eapply ST.heq_ex. intros.
-            unfold tvar in *. generalize (HCons v h). intros.
-            eapply ST.heq_star_comm.
-            specialize (IHy 
-              
-            
-        
-          
-          (** TODO: This is problematic because existsEach only generalizes the
-           ** top list of variables, so we can't state a commutativity lemma
-           **)
-
-      
-      Admitted.
+          intros. unfold heq; simpl. rewrite liftSExpr_existsEach.
+          match goal with
+            | [ |- ?G ] => change G with (heq A A (hlist_app Z C) cs (Star P (existsEach y (x ++ z) (liftSExpr y x z Q))) (existsEach y (x ++ z) (Star (liftSExpr nil y (x ++ z) P) (liftSExpr y x z Q))))
+          end.
+          apply heq_star_comm. etransitivity. apply lift_existsEach_star.
+          eapply existsEach_heq. intros. apply heq_star_comm. reflexivity.
+      Qed.
 
       Lemma lift_denote_lift : forall u a b c (s : SHeap u (a ++ c)) X Y,
         heq X X Y cs (liftSExpr a b c (denote s)) (denote (liftSHeap a b c s)).
       Proof. Admitted.
 
+      Lemma starred_Star : forall u v T (F : T -> sexpr fs sfuncs u v) a b X Y,
+        heq X X Y cs (starred F (a ++ b)) (Star (starred F a) (starred F b)).
+      Proof.
+        clear. induction a; simpl.
+          intros. symmetry. apply heq_star_emp. reflexivity.
+          intros. symmetry. apply heq_star_assoc. apply heq_star_frame. reflexivity.
+          symmetry. eauto.
+      Qed.
+
+       Ltac cancel_heq :=
+         repeat apply heq_star_assoc;
+           symmetry; (repeat apply heq_star_assoc; 
+             (apply heq_star_frame; [ reflexivity | ]) || apply heq_star_comm).
 
       Lemma denote_join : forall a b (P Q : SHeap a b) X Y,
         heq X X Y cs (denote (join_SHeap P Q)) (Star (denote P) (denote Q)).
       Proof.
         clear. unfold join_SHeap. destruct P; destruct Q; simpl in *. 
-        unfold denote; simpl.
+        unfold denote; simpl. intros. etransitivity.
+        instantiate (1 := Star
+          (Star (dmap_fold
+            (fun (a0 : sexpr fs sfuncs a b) (x : fin sfuncs)
+               (y : list (hlist (expr fs a b) (SDomain (get sfuncs x)))) =>
+             fold_left
+               (fun (a1 : sexpr fs sfuncs a b)
+                  (y0 : hlist (expr fs a b) (SDomain (get sfuncs x))) =>
+                Star (Func x y0) a1) y a0) Emp funcs0)
+          (dmap_fold
+            (fun (a0 : sexpr fs sfuncs a b) (x : fin sfuncs)
+               (y : list (hlist (expr fs a b) (SDomain (get sfuncs x)))) =>
+             fold_left
+               (fun (a1 : sexpr fs sfuncs a b)
+                  (y0 : hlist (expr fs a b) (SDomain (get sfuncs x))) =>
+                Star (Func x y0) a1) y a0) Emp funcs1))
+          (Star (Star (fold_right
+               (fun (x : expr fs a b None) (a0 : sexpr fs sfuncs a b) =>
+                Star (Inj x) a0) Emp pures0) (fold_right
+               (fun (x : expr fs a b None) (a0 : sexpr fs sfuncs a b) =>
+                Star (Inj x) a0) Emp pures1))
+          (Star (fold_right
+               (fun (x : ST.hprop (tvarD pcType) (tvarD stateType) nil)
+                 (a0 : sexpr fs sfuncs a b) => Star (Const x) a0) Emp other0)
+          (fold_right
+            (fun (x : ST.hprop (tvarD pcType) (tvarD stateType) nil)
+              (a0 : sexpr fs sfuncs a b) => Star (Const x) a0) Emp other1)))).
+       Focus 2.
+       repeat (reflexivity || cancel_heq). 
+        apply heq_star_frame; [ | apply heq_star_frame ]; try eapply starred_Star.
+        (** TODO: this is the annoying case **)
+
       Admitted.
 
       Theorem denote_hash_left : forall G (s : sexpr fs sfuncs _ _), 
@@ -657,10 +731,9 @@ refine (
           (** Exists **)
           Focus.
           intros. simpl. destruct (hash_left s); simpl in *.
-            etransitivity. 2: symmetry; eapply existsEach_peel_back.
-            instantiate (1 := denote s0). eapply heq_ex. eauto.
-            intros. clear IHs. generalize (hlist_app Z G). generalize s0. clear. uip_all. 
-            generalize s0 h e e0. simpl in *. uip_all. unfold eq_rect_r, eq_rect; simpl.
+            rewrite existsEach_peel_back. eapply heq_ex. intros.
+            etransitivity. eapply IHs. eapply existsEach_heq. intros.
+            uip_all. generalize e e0. simpl in *. uip_all. unfold eq_rect_r, eq_rect; simpl.
             reflexivity.
 
           (** Func **)
@@ -819,896 +892,3 @@ End SepExpr.
 
 Require Export Expr.
 
-(*
-    Section WithCS.
-    Variable cs : codeSpec (tvarD pcType) (tvarD stateType).
-
-    Ltac cancel_all :=
-      let s :=
-        (   reflexivity 
-         || simple apply ST.himp_star_emp_c
-         || simple apply ST.himp_star_emp_p
-         || simple apply ST.heq_star_emp
-         || (symmetry; simple apply ST.heq_star_emp; symmetry)
-         || simple apply ST.himp_star_cancel
-         || simple apply ST.heq_star_cancel
-        )
-      in
-      let perm :=
-        try ((eapply ST.himp_star_comm_p; repeat simple apply ST.himp_star_assoc_p) || 
-             (eapply ST.heq_star_comm; symmetry; repeat simple apply ST.heq_star_assoc; symmetry)); 
-        try do 10 (s || 
-          match goal with
-            | [ |- ST.heq _ _ _ _ _ ] =>
-              symmetry; simple apply ST.heq_star_comm; symmetry; repeat simple apply ST.heq_star_assoc
-            | [ |- ST.himp _ _ _ _ _ ] =>
-              repeat (simple apply ST.himp_star_assoc_c)
-          end)
-      in
-      do 10 perm.
-
-    Theorem denote_hash : forall G s cs, 
-      heq G cs s (existsEach (projT1 (hash s)) nil (denote (projT2 (hash s)))).
-    Proof.
-      clear. induction s; unfold denote, heq; simpl; intros.
-        cancel_all.
-        cancel_all.
-        admit.
-        admit.
-        cancel_all.
-        cancel_all.
-    Admitted.
-
-
-    Lemma fold_star : forall K V vars G (ctor : forall k : K, V k -> sexpr fs sfuncs vars) (B : @dmap K V) P Q,
-      heq G cs 
-        (Star Q (dmap_fold (fun (a : sexpr fs sfuncs vars) (k : K) (v : V k) => Star (ctor k v) a) P B))
-        (Star P (dmap_fold (fun (a : sexpr fs sfuncs vars) (k : K) (v : V k) => Star (ctor k v) a) Q B)).
-    Proof.
-      induction B; unfold heq in *; simpl in *; intros. cancel_all.
-      etransitivity. eapply IHB2. etransitivity. 2: eapply IHB2.
-      etransitivity. eapply ST.heq_star_frame. etransitivity; [ | apply (IHB1 (Star (ctor k v) P) Emp); simpl ]; cancel_all.
-      etransitivity; [ | apply (IHB2 Q Emp) ]; cancel_all.
-      etransitivity. Focus 2.
-      eapply ST.heq_star_frame. etransitivity; [ eapply (IHB1 Emp (Star (ctor k v) Q)) | ]; cancel_all.
-      etransitivity; [ eapply (IHB2 Emp P) | ]; cancel_all. simpl; cancel_all.
-    Qed.
-
-    Lemma fold_star' : forall K V vars G (ctor : forall k : K, V k -> sexpr fs sfuncs vars) (B : @dmap K V) P,
-      heq G cs 
-        (dmap_fold (fun (a : sexpr fs sfuncs vars) (k : K) (v : V k) => Star (ctor k v) a) P B)
-        (Star P (dmap_fold (fun (a : sexpr fs sfuncs vars) (k : K) (v : V k) => Star (ctor k v) a) Emp B)).
-    Proof.
-      intros. etransitivity; [ | eapply fold_star ]. unfold heq; simpl; cancel_all.
-    Qed.
-
-    Lemma fold_star'' : forall K V vars G (ctor : forall k : K, V k -> sexpr fs sfuncs vars) (B : @dmap K V) P,
-      heq G cs
-        (Star P (dmap_fold (fun (a : sexpr fs sfuncs vars) (k : K) (v : V k) => Star (ctor k v) a) Emp B))
-        (dmap_fold (fun (a : sexpr fs sfuncs vars) (k : K) (v : V k) => Star (ctor k v) a) P B).
-    Proof.
-      intros. etransitivity; [ eapply fold_star | ]; unfold heq; simpl; cancel_all.
-    Qed.
-
-    Lemma star_insert : forall K V vars G (ctor : forall k : K, V k -> sexpr fs sfuncs vars)
-      (cmp : forall a b : K, option (dcomp a b)) (B : @dmap K V) k (v : V k) P,
-      heq G cs
-        (dmap_fold
-          (fun (a : sexpr fs sfuncs vars) (k : K) (v : V k) =>
-            Star (ctor k v) a) P (@dmap_insert _ _ cmp k v B))
-        (Star
-          (dmap_fold
-            (fun (a : sexpr fs sfuncs vars) (k : K) (v : V k) => Star (ctor k v) a) P B) (ctor k v)).
-    Proof.      
-      clear. induction B. simpl. intros. cancel_all. 
-      simpl. intros. destruct (cmp k k0). destruct d; simpl in *. etransitivity; [ eapply fold_star' | ].
-      unfold heq in *; simpl in *.
-    Admitted.
-
-(*
-    Lemma denote_hash_rec : forall vars (s : sexpr fs sfuncs consts vars) P (cc : _ -> _ -> _ -> _ -> _ -> SHeap vars) G,
-      (forall A B C D E, 
-        heq stateMem G cs 
-          (denote (cc D E A B C))
-          (Star P (denote (Build_SHeap D E A B C)))) ->
-      forall A B C D E,
-      heq stateMem G cs (denote (hash_rec s cc A B C D E)) (Star (Star (denote (Build_SHeap A B C D E)) P) s).
-    Proof.
-      unfold hash_cc, Himp; do 2 intro. unfold heq.
-      induction s; intros; simpl; instantiate.
-(*
-        try solve [ cancel_all; eauto | etransitivity; [ eapply H | ]; unfold denote; simpl; do 5 cancel_all ].
-        (* Star *)
-        etransitivity. eapply IHs1. intros. etransitivity. eapply IHs2. intros. etransitivity. eapply H. reflexivity.
-        instantiate (1 := Star P s2). cancel_all. repeat cancel_all.
-        (* Cptr *) Focus.
-        etransitivity. eapply H. unfold denote; simpl. cancel_all. apply star_comm_p. cancel_all. cancel_all.
-        clear.
-        match goal with
-          | [ |- context [ @Emp ?A ?B ?C ?D ?E ?F ?G ] ] => generalize (@Emp A B C D E F G)
-        end. induction B; intros; simpl. apply star_comm_p. reflexivity. etransitivity. unfold fmap_fold. eapply fold_star'.
-        etransitivity. eapply star_frame. eapply IHB1. reflexivity. cancel_all. etransitivity. eapply star_frame.
-        unfold fmap_fold. eapply fold_star'. reflexivity. cancel_all. etransitivity. 2: eapply star_frame.
-        2: unfold fmap_fold; eapply fold_star''. 2: reflexivity. apply star_assoc_c. etransitivity.
-        2: eapply star_frame. 2: eapply fold_star''. 2: reflexivity. cancel_all.
-        (** Func **) Focus.
-*)
-    Admitted.
-
-    Lemma denote_hash_rec' : forall vars (s : sexpr fs sfuncs consts vars) P (cc : _ -> _ -> _ -> _ -> _ -> SHeap vars) G,
-      (forall A B C D E, 
-        himp stateMem G cs 
-          (Star P (denote (Build_SHeap D E A B C)))
-          (denote (cc D E A B C))) ->
-      forall A B C D E,
-      himp stateMem G cs (Star (Star (denote (Build_SHeap A B C D E)) P) s) (denote (hash_rec s cc A B C D E)).
-    Proof.
-    Admitted.
-
-
-
-    Theorem denote_hash_cc : forall (s : sexpr fs sfuncs consts nil),
-      Heq stateMem cs (denote (hash_cc s (@Build_SHeap nil))) s.
-    Proof.
-      unfold Himp. intros. unfold hash_cc. etransitivity. eapply denote_hash_rec.
-      instantiate (1 := Emp). intros. 
-      generalize (denote {| funcs := D; cptrs := E; pures := A; cnsts := B; other := C |}). unfold heq; simpl.
-      intros; cancel_all. unfold denote. simpl. unfold Heq, heq; simpl.
-      do 10 (try apply ST.heq_star_comm; symmetry; repeat apply ST.heq_star_assoc; symmetry; try apply ST.heq_star_emp).
-      reflexivity.
-    Qed.
-*)
-
-
-    (** Procedure:
-     ** - Hash the left hand side
-     ** - ?? Handle implications...
-     ** - ?? Generate <> constraints ??
-     ** - For each right hand side conjunct
-     **   - if it is in the SHeap
-     **       cancel
-     **     else 
-     **       ?? is this automatically problematic, this procedure probably won't prove it
-     ** - Discharge pure constraints with solver...
-     **)
-
-(*
-    Goal forall cs (a : fin consts), 
-      Himp stateMem cs (Const fs sfuncs nil a) (Const fs sfuncs nil a).
-      intros.
-      pose (ReflSep cs nil (Const _ _ nil a) (Const _ _ nil a)). simpl in *.
-      (** Note: everything has to be concrete in order for simplification to work! **)
-      unfold ReflSep in *. unfold sexprCmp in *.
-      destruct (finCmp a a). simpl in *. 
-      match goal with
-        | [ H := Some ?X |- _ ] => generalize X
-      end. auto.
-      congruence.
-    Defined.
-*)
-
-   Section TakeOut.
-      Context {T : Type}.
-      Variable Teq : T -> T -> bool.
-      
-      Require Import List.
-      Fixpoint take_out (v : T) (ls : list T) (r : list T): option (list T) :=
-        match ls with
-          | nil => None
-          | a :: b => if Teq a v then Some (r ++ b) else take_out v b (a :: r)
-        end.
-    End TakeOut.
-
-
-    Fixpoint All vars (ls : list (expr fs vars None)) : hlist (@tvarD _) vars -> Prop :=
-      match ls with
-        | nil => fun _ => True
-        | a :: b => fun G => exprD G a /\ All b G
-      end.
-
-    (** TODO: 
-     ** - cancel with unification
-     ** - 
-     **)
-    
-
-    (** Eliminate e from the symbolic heap and return the set of pure facts that 
-     ** imply the conclusion
-     **)
-    Fixpoint sepCancel vars (e : sexpr fs sfuncs vars) {struct e}
-      : SHeap vars -> SHeap vars -> SHeap vars * SHeap vars :=
-      match e in sexpr _ _ vars 
-        return SHeap vars -> SHeap vars -> SHeap vars * SHeap vars
-        with
-        | Emp _ => fun h rem => (h, rem)
-        | Func _ f a => fun h rem =>
-          match dmap_remove (fun x y => Some (@finCmp _ _ x y)) f (funcs h) with
-            | Some (ls, fs') => 
-              match take_out (fun x y => if hlistEq (@exprEq _ _ _ ) x y then true else false) a ls nil with
-                | None => (h,rem)
-                | Some nil => 
-                  ({| funcs := fs' 
-                    ; pures := pures h
-                    ; other := other h
-                    |}, rem)
-                | Some v =>
-                  ({| funcs := dmap_insert (fun x y => Some (@finCmp _ _ x y)) f v fs'
-                    ; pures := pures h
-                    ; other := other h
-                    |}, rem)
-              end
-            | None => (h,rem)
-          end              
-(*
-          match fmap_remove (@exprCmp _ _ _ _) p (cptrs h) with
-            | Some (s', cp') => 
-              match sexprCmp s s' with
-                | Some (Env.Eq _) => 
-                ({| funcs := funcs h 
-                  ; cptrs := cp'
-                  ; pures := pures h
-                  ; other := other h
-                  ; cnsts := cnsts h
-                  |}, rem)
-                | _ => (h,rem)
-              end
-           | None => (h,rem)
-          end
-*)
-        | Star _ l r => fun h rem =>
-          let '(h',rem') := sepCancel l h rem in
-          sepCancel r h' rem'
-        | _ => fun h rem => (h,rem)
-      end.
-    
-    Lemma sepCancel_cancels' : forall vars G e h r rl rr,
-      @sepCancel vars e h r = (rl, rr) ->
-      forall P,
-      himp G cs (denote rl) (Star (denote rr) P) ->
-      himp G cs (denote h) (Star (Star e (denote r)) P).
-    Proof.
-(*
-      induction e; simpl; intros;
-        repeat match goal with
-                 | [ H : (_,_) = (_,_) |- _ ] => inversion H; clear H; subst
-                 | [ H : sepCancel _ _ _ = (_,_) , H' : _ |- _ ] => apply H' in H; clear H'
-               end;
-        try solve [ etransitivity; [ eassumption | ]; do 5 cancel_all ].
-      Focus 2.
-      (* star *)
-      case_eq (sepCancel e1 h r). intros. rewrite H1 in *.
-      specialize (@IHe1 G _ _ _ _ H1).
-      specialize (@IHe2 G _ _ _ _ H). 
-      etransitivity. eapply IHe1. etransitivity. eapply IHe2. eassumption.
-      instantiate (1 := (Star e2 P)). generalize (denote s0); intros; cancel_all.
-      generalize (denote r); intros; cancel_all.
-*)
-    Admitted.
-
-    Theorem sepCancel_cancels : forall e h rl rr,
-      sepCancel e h (SHeap_empty nil) = (rl, rr) ->
-      Himp cs (denote rl) (denote rr) ->
-      Himp cs (denote h) e.
-    Proof.
-      unfold Himp; intros. etransitivity. eapply sepCancel_cancels'. eassumption.
-      instantiate (1 := Emp). etransitivity. eassumption. generalize (denote rr).
-      intros; cancel_all. unfold denote. simpl. 
-      repeat (apply star_comm_p; repeat apply star_assoc_p; apply star_emp_p).
-      unfold himp; simpl. cancel_all.
-    Qed.
-  
-  End WithCS.
-
-    Definition CancelSep : @SProverT types fs pcType stateType sfuncs.
-(*
-    red. refine (fun _ _ gl gr =>
-      match hash gl , hash gr with
-        | existT ql lhs , existT qr rhs =>
-          match sepCancel gr lhs (SHeap_empty _) as k 
-            return sepCancel gr lhs (SHeap_empty _) = k -> _ with
-            | (lhs',rhs') => fun pf =>
-              @existT _ _ (denote lhs', denote rhs') _
-          end (eq_refl _)
-      end).
-      intros. etransitivity. 2: eapply sepCancel_cancels. 2: eassumption. 2: eauto.
-      unfold lhs. etransitivity. eapply denote_hash_cc. unfold Himp, himp. reflexivity.
-*)
-    Admitted.
-
-  End BabySep.
-
-  (** Tests **)
-  Section ProverTests.
-    Require Import Arith.
-    Variable pcType : Type.
-    Variable stateType : Type.
-
-    Definition types := 
-      {| Impl := pcType ; Eq := fun _ _ => None |} ::
-      {| Impl := stateType ; Eq := fun _ _ => None |} ::
-      {| Impl := nat; Eq := fun x y => match eq_nat_dec x y with left Heq => Some Heq | _ => None end |} :: nil.
-
-    Definition fs : functions types :=
-       {| Domain := Some (FS (FS FO)) :: Some (FS (FS FO)) :: nil;
-          Range := None; Denotation := eq |}
-    :: {| Domain := (Some (FS (FS FO)) :: Some (FS (FS FO)) :: nil) : list (tvar types);
-          Range := Some (FS (FS FO)); Denotation := plus |}
-    :: nil.
-
-    Definition pcTypeV : tvar types := Some FO.
-    Definition stateTypeV : tvar types := Some (FS FO).
-
-    Definition consts : list (PropX (tvarD pcTypeV) (tvarD stateTypeV)) := nil.
-    Definition vars : variables types := nil.
-
-    Parameter repr : nat -> ST.Hprop (tvarD pcTypeV) (tvarD stateTypeV).
-
-    Variable stateMem : tvarD stateTypeV -> B.mem.
-    Definition sfuncs : list (@ssignature types pcTypeV stateTypeV) :=
-      {| SDomain := Some (FS (FS FO)) :: nil
-       ; SDenotation := repr
-         : functionTypeD (map (@tvarD types) (Some (FS (FS FO)) :: nil)) (ST.Hprop (tvarD pcTypeV) (tvarD stateTypeV))
-       |} :: nil.
-
-  Goal forall cs,
-    Himp cs (@Func types fs pcTypeV stateTypeV sfuncs vars FO (HCons (Expr.Const fs vars (Some (FS (FS FO))) 1) HNil))
-            (@Func types fs pcTypeV stateTypeV sfuncs vars FO (HCons (Expr.Const fs vars (Some (FS (FS FO))) 1) HNil)).
-  Proof.
-    intros.
-    (*
-    match goal with
-      | [ |- Himp ?M ?C ?L ?R ] =>
-        let R := fresh in
-        let rr := eval hnf in (@CancelSep types fs pcTypeV stateTypeV M sfuncs C nil L R) in
-        match rr with
-          | existT _ ?PF => apply PF; unfold denote; simpl
-        end
-    end. unfold Himp, himp. reflexivity.
-*)
-    Admitted.
-  End ProverTests.
-  
-  Section QSexpr.
-    (** Guarded separation logic expressions **)
-  End QSexpr.
-*)
-
-
-
-(*
-    Definition hash_rec vars'' vars (s : sexpr fs sfuncs vars) 
-      :  (forall vs,
-             @dmap (fin sfuncs) (fun f => list (hlist (expr fs (vs ++ vars)) (SDomain (get sfuncs f))))
-          -> list (expr fs (vs ++ vars) None)
-          -> list (ST.Hprop (tvarD pcType) (tvarD stateType))
-          -> { vars' : variables types & SHeap (vars' ++ vs ++ vars) })
-      -> @dmap (fin sfuncs) (fun f => list (hlist (expr fs (vars'' ++ vars)) (SDomain (get sfuncs f))))
-      -> list (expr fs (vars'' ++ vars) None)
-      -> list (ST.Hprop (tvarD pcType) (tvarD stateType))
-      -> { vars' : variables types & SHeap (vars' ++ vars'' ++ vars) }.
-    refine ((fix hash_rec vars (s : sexpr fs sfuncs vars) 
-      :  forall vars'', (forall vs,
-             @dmap (fin sfuncs) (fun f => list (hlist (expr fs (vs ++ vars)) (SDomain (get sfuncs f))))
-          -> list (expr fs (vs ++ vars) None)
-          -> list (ST.Hprop (tvarD pcType) (tvarD stateType))
-          -> { vars' : variables types & SHeap (vars' ++ vs ++ vars) })
-      -> @dmap (fin sfuncs) (fun f => list (hlist (expr fs (vars'' ++ vars)) (SDomain (get sfuncs f))))
-      -> list (expr fs (vars'' ++ vars) None)
-      -> list (ST.Hprop (tvarD pcType) (tvarD stateType))
-      -> { vars' : variables types & SHeap (vars' ++ vars'' ++ vars) } :=
-      match s in @sexpr _ _ _ _ _ vs 
-        return forall vars'',
-           (forall vs', 
-               @dmap (fin sfuncs) (fun f => list (hlist (expr fs (vs' ++ vs)) (SDomain (get sfuncs f))))
-            -> list (expr fs (vs' ++ vs) None)
-            -> list (ST.Hprop (tvarD pcType) (tvarD stateType))
-            -> { vars' : variables types & SHeap (vars' ++ vs' ++ vs) })
-        -> @dmap (fin sfuncs) (fun f => list (hlist (expr fs (vars'' ++ vs)) (SDomain (get sfuncs f))))
-        -> list (expr fs (vars'' ++ vs) None)
-        -> list (ST.Hprop (tvarD pcType) (tvarD stateType))
-        -> { vars' : variables types & SHeap (vars' ++ vars'' ++ vs) }
-        with
-        | Emp vars => fun vars'' cc => _
-        | Inj _ p => fun cc fs ps ot =>
-          _ (*cc nil fs (p :: ps) ot  *)
-        | Star _ l r => fun cc => _
-(*          hash_rec l (fun vs => hash_rec (liftSExpr vs r) cc () () () *)
-        | Func _ f args => fun cc fs ps ot => _
-(*
-          match dmap_remove (fun a b => Some (@finCmp _ _ a b)) f fs with
-            | None =>
-              cc (dmap_insert (fun a b => Some (@finCmp _ _ a b)) f (args :: nil) fs) ps ot
-            | Some (v,fs') =>
-              cc (dmap_insert (fun a b => Some (@finCmp _ _ a b)) f (args :: v) fs') ps ot
-          end
-*)
-        | Exists vv t b => fun cc fs' ps ot => _
-        | Const _ x => fun cc fs ps ot =>
-          _ (* cc nil fs ps (x :: ot) *)
-      end) vars s vars'').
-    Focus.
-    intros. eapply cc.
-    
-
-    Definition hash_rec vars (s : sexpr fs sfuncs vars) 
-      :  (forall vs,
-             @dmap (fin sfuncs) (fun f => list (hlist (expr fs (vs ++ vars)) (SDomain (get sfuncs f))))
-          -> list (expr fs (vs ++ vars) None)
-          -> list (ST.Hprop (tvarD pcType) (tvarD stateType))
-          -> { vars' : variables types & SHeap (vars' ++ vs ++ vars) })
-      -> @dmap (fin sfuncs) (fun f => list (hlist (expr fs vars) (SDomain (get sfuncs f))))
-      -> list (expr fs vars None)
-      -> list (ST.Hprop (tvarD pcType) (tvarD stateType))
-      -> { vars' : variables types & SHeap (vars' ++ vars) }.
-    revert s; revert vars.
-    refine (Fix hash_rec vars (s : sexpr fs sfuncs vars) {struct s}
-      :  (forall vs,
-             @dmap (fin sfuncs) (fun f => list (hlist (expr fs (vs ++ vars)) (SDomain (get sfuncs f))))
-          -> list (expr fs (vs ++ vars) None)
-          -> list (ST.Hprop (tvarD pcType) (tvarD stateType))
-          -> { vars' : variables types & SHeap (vars' ++ vs ++ vars) })
-      -> @dmap (fin sfuncs) (fun f => list (hlist (expr fs vars) (SDomain (get sfuncs f))))
-      -> list (expr fs vars None)
-      -> list (ST.Hprop (tvarD pcType) (tvarD stateType))
-      -> { vars' : variables types & SHeap (vars' ++ vars) } :=
-      match s in @sexpr _ _ _ _ _ vs 
-        return 
-           (forall vs', 
-               @dmap (fin sfuncs) (fun f => list (hlist (expr fs (vs' ++ vs)) (SDomain (get sfuncs f))))
-            -> list (expr fs (vs' ++ vs) None)
-            -> list (ST.Hprop (tvarD pcType) (tvarD stateType))
-            -> { vars' : variables types & SHeap (vars' ++ vs' ++ vs) })
-        -> @dmap (fin sfuncs) (fun f => list (hlist (expr fs vs) (SDomain (get sfuncs f))))
-        -> list (expr fs vs None)
-        -> list (ST.Hprop (tvarD pcType) (tvarD stateType))
-        -> { vars' : variables types & SHeap (vars' ++ vs) }
-        with
-        | Emp vars => fun cc => cc nil
-        | Inj _ p => fun cc fs ps ot =>
-          cc nil fs (p :: ps) ot 
-        | Star vv l r => fun cc =>
-          let cc' vs :=
-            hash_rec (vs ++ vv) (liftSExpr nil vs vv r)
-            (fun vs' => match app_ass _ _ _ in _ = t 
-                          return 
-                          dmap (fin sfuncs)
-                          (fun f : fin sfuncs =>
-                            list (hlist (expr fs t) (SDomain (get sfuncs f)))) ->
-                          list (expr fs t None) ->
-                          list (ST.Hprop (tvarD pcType) (tvarD stateType)) ->
-                          {vars' : variables types & SHeap (vars' ++ t)}
-                          with
-                          | refl_equal => cc (vs' ++ vs)
-                        end)
-          in
-          hash_rec _ l cc'
-        | Func _ f args => fun cc fs ps ot => _
-(*
-          match dmap_remove (fun a b => Some (@finCmp _ _ a b)) f fs with
-            | None =>
-              cc (dmap_insert (fun a b => Some (@finCmp _ _ a b)) f (args :: nil) fs) ps ot
-            | Some (v,fs') =>
-              cc (dmap_insert (fun a b => Some (@finCmp _ _ a b)) f (args :: v) fs') ps ot
-          end
-*)
-        | Exists vv t b => fun cc fs' ps ot => 
-          let cc := fun vs =>
-            match pf_list_simpl t vv vs in _ = t' 
-              return dmap (fin sfuncs)
-              (fun f : fin sfuncs => list (hlist (expr fs t') (SDomain (get sfuncs f)))) ->
-              list (expr fs t' None) ->
-              list (ST.Hprop (tvarD pcType) (tvarD stateType)) ->
-              {vars' : variables types & SHeap (vars' ++ t')}
-              with
-              | refl_equal => @cc (vs ++ t :: nil)
-            end
-          in
-          let fs' := dmap_map _ _ _ (fun t' => @List.map _ _ (@hlist_map _ _ _ (liftExpr vv (t :: nil) nil) _)) fs' in
-          let ps' := map (liftExpr vv (t :: nil) nil (T := None)) ps in
-          match hash_rec _ b cc fs' ps' ot with
-            | existT a b => @existT _ _ (a ++ t :: nil) match eq_sym (pf_list_simpl t vv a) in _ = t' return SHeap t' with
-                                                          | refl_equal => b
-                                                        end
-          end
-        | Const _ x => fun cc fs ps ot =>
-          cc nil fs ps (x :: ot)
-      end).
-
-    Definition hash_rec vars (s : sexpr fs sfuncs vars) 
-      :  (forall vs,
-             @dmap (fin sfuncs) (fun f => list (hlist (expr fs (vs ++ vars)) (SDomain (get sfuncs f))))
-          -> list (expr fs (vs ++ vars) None)
-          -> list (ST.Hprop (tvarD pcType) (tvarD stateType))
-          -> { vars' : variables types & SHeap (vars' ++ vs ++ vars) })
-      -> @dmap (fin sfuncs) (fun f => list (hlist (expr fs vars) (SDomain (get sfuncs f))))
-      -> list (expr fs vars None)
-      -> list (ST.Hprop (tvarD pcType) (tvarD stateType))
-      -> { vars' : variables types & SHeap (vars' ++ vars) }.
-    revert s; revert vars.
-    refine (fix hash_rec vars (s : sexpr fs sfuncs vars) {struct s}
-      :  (forall vs,
-             @dmap (fin sfuncs) (fun f => list (hlist (expr fs (vs ++ vars)) (SDomain (get sfuncs f))))
-          -> list (expr fs (vs ++ vars) None)
-          -> list (ST.Hprop (tvarD pcType) (tvarD stateType))
-          -> { vars' : variables types & SHeap (vars' ++ vs ++ vars) })
-      -> @dmap (fin sfuncs) (fun f => list (hlist (expr fs vars) (SDomain (get sfuncs f))))
-      -> list (expr fs vars None)
-      -> list (ST.Hprop (tvarD pcType) (tvarD stateType))
-      -> { vars' : variables types & SHeap (vars' ++ vars) } :=
-      match s in @sexpr _ _ _ _ _ vs 
-        return 
-           (forall vs', 
-               @dmap (fin sfuncs) (fun f => list (hlist (expr fs (vs' ++ vs)) (SDomain (get sfuncs f))))
-            -> list (expr fs (vs' ++ vs) None)
-            -> list (ST.Hprop (tvarD pcType) (tvarD stateType))
-            -> { vars' : variables types & SHeap (vars' ++ vs' ++ vs) })
-        -> @dmap (fin sfuncs) (fun f => list (hlist (expr fs vs) (SDomain (get sfuncs f))))
-        -> list (expr fs vs None)
-        -> list (ST.Hprop (tvarD pcType) (tvarD stateType))
-        -> { vars' : variables types & SHeap (vars' ++ vs) }
-        with
-        | Emp vars => fun cc => cc nil
-        | Inj _ p => fun cc fs ps ot =>
-          cc nil fs (p :: ps) ot 
-        | Star vv l r => fun cc =>
-          let cc' vs :=
-            hash_rec (vs ++ vv) (liftSExpr nil vs vv r)
-            (fun vs' => match app_ass _ _ _ in _ = t 
-                          return 
-                          dmap (fin sfuncs)
-                          (fun f : fin sfuncs =>
-                            list (hlist (expr fs t) (SDomain (get sfuncs f)))) ->
-                          list (expr fs t None) ->
-                          list (ST.Hprop (tvarD pcType) (tvarD stateType)) ->
-                          {vars' : variables types & SHeap (vars' ++ t)}
-                          with
-                          | refl_equal => cc (vs' ++ vs)
-                        end)
-          in
-          hash_rec _ l cc'
-        | Func _ f args => fun cc fs ps ot => _
-(*
-          match dmap_remove (fun a b => Some (@finCmp _ _ a b)) f fs with
-            | None =>
-              cc (dmap_insert (fun a b => Some (@finCmp _ _ a b)) f (args :: nil) fs) ps ot
-            | Some (v,fs') =>
-              cc (dmap_insert (fun a b => Some (@finCmp _ _ a b)) f (args :: v) fs') ps ot
-          end
-*)
-        | Exists vv t b => fun cc fs' ps ot => 
-          let cc := fun vs =>
-            match pf_list_simpl t vv vs in _ = t' 
-              return dmap (fin sfuncs)
-              (fun f : fin sfuncs => list (hlist (expr fs t') (SDomain (get sfuncs f)))) ->
-              list (expr fs t' None) ->
-              list (ST.Hprop (tvarD pcType) (tvarD stateType)) ->
-              {vars' : variables types & SHeap (vars' ++ t')}
-              with
-              | refl_equal => @cc (vs ++ t :: nil)
-            end
-          in
-          let fs' := dmap_map _ _ _ (fun t' => @List.map _ _ (@hlist_map _ _ _ (liftExpr vv (t :: nil) nil) _)) fs' in
-          let ps' := map (liftExpr vv (t :: nil) nil (T := None)) ps in
-          match hash_rec _ b cc fs' ps' ot with
-            | existT a b => @existT _ _ (a ++ t :: nil) match eq_sym (pf_list_simpl t vv a) in _ = t' return SHeap t' with
-                                                          | refl_equal => b
-                                                        end
-          end
-        | Const _ x => fun cc fs ps ot =>
-          cc nil fs ps (x :: ot)
-      end).
-    Focus.
-    refine (
-          let cc' vs :=
-            hash_rec (vs ++ vv) (liftSExpr nil vs vv r)
-            (fun vs' => match app_ass _ _ _ in _ = t 
-                          return 
-                          dmap (fin sfuncs)
-                          (fun f : fin sfuncs =>
-                            list (hlist (expr fs t) (SDomain (get sfuncs f)))) ->
-                          list (expr fs t None) ->
-                          list (ST.Hprop (tvarD pcType) (tvarD stateType)) ->
-                          {vars' : variables types & SHeap (vars' ++ t)}
-                          with
-                          | refl_equal => cc (vs' ++ vs)
-                        end)
-          in
-          hash_rec _ l cc'
-
-).
-    
-
-
-    Definition hash_cc vars (s : sexpr fs sfuncs vars)
-      (cc : @dmap (fin sfuncs) (fun f => list (hlist (expr fs vars) (SDomain (get sfuncs f))))
-       -> list (expr fs vars None)
-       -> list (sexpr fs sfuncs vars) -> { vars' : variables types & SHeap (vars' ++ vars) }) : 
-      { vars' : variables types & SHeap (vars' ++ vars) } :=
-      @hash_rec vars s cc dmap_empty nil nil.
-
-    Fixpoint existsEach (vars vars' : variables types) 
-      : sexpr fs sfuncs (vars ++ vars') -> sexpr fs sfuncs vars' :=
-      match vars as vars return sexpr fs sfuncs (vars ++ vars') -> sexpr fs sfuncs vars'
-        with
-        | nil => fun s => s
-        | a :: b => fun s => @existsEach b vars' (Exists a s)
-      end.
-*)
-
-(*
-      Fixpoint sepCancel vars (e : sexpr fs sfuncs vars) {struct e}
-        : SHeap vars -> SHeap vars -> SHeap vars * SHeap vars.
-      match e in sexpr _ _ vars 
-        return SHeap vars -> SHeap vars -> SHeap vars * SHeap vars
-        with
-        | Emp _ => fun h rem => (h, rem)
-        | Func _ f a => fun h rem =>
-          match dmap_remove (fun x y => Some (@finCmp _ _ x y)) f (funcs h) with
-            | Some (ls, fs') => 
-              match take_out (fun x y => if hlistEq (@exprEq _ _ _ ) x y then true else false) a ls nil with
-                | None => (h,rem)
-                | Some nil => 
-                  ({| funcs := fs' 
-                    ; pures := pures h
-                    ; other := other h
-                    |}, rem)
-                | Some v =>
-                  ({| funcs := dmap_insert (fun x y => Some (@finCmp _ _ x y)) f v fs'
-                    ; pures := pures h
-                    ; other := other h
-                    |}, rem)
-              end
-            | None => (h,rem)
-          end              
-(*
-          match fmap_remove (@exprCmp _ _ _ _) p (cptrs h) with
-            | Some (s', cp') => 
-              match sexprCmp s s' with
-                | Some (Env.Eq _) => 
-                ({| funcs := funcs h 
-                  ; cptrs := cp'
-                  ; pures := pures h
-                  ; other := other h
-                  ; cnsts := cnsts h
-                  |}, rem)
-                | _ => (h,rem)
-              end
-           | None => (h,rem)
-          end
-*)
-        | Star _ l r => fun h rem =>
-          let '(h',rem') := sepCancel l h rem in
-          sepCancel r h' rem'
-        | _ => fun h rem => (h,rem)
-      end.
-*)
-
-
-
-          
-(*
-          match sepCancel gr lhs (SHeap_empty _) as k 
-            return sepCancel gr lhs (SHeap_empty _) = k -> _ with
-            | (lhs',rhs') => fun pf =>
-              @existT _ _ (denote lhs', denote rhs') _
-          end (eq_refl _)
-*)
-(*
-      end).
-      intros. etransitivity. 2: eapply sepCancel_cancels. 2: eassumption. 2: eauto.
-      unfold lhs. etransitivity. eapply denote_hash_cc. unfold Himp, himp. reflexivity.
-*)
-
-(*
-    Fixpoint hash vars (s : sexpr fs sfuncs nil vars) :
-      { vars' : variables types & SHeap vars' vars }.
-    refine (
-      match s in sexpr _ _ _ vars return { vars' : variables types & SHeap vars' vars } with
-        | Emp _ => @existT _ _ nil (SHeap_empty _ _)
-        | Inj _ p => @existT _ _ nil
-          {| funcs := dmap_empty
-           ; pures := p :: nil
-           ; other := nil
-           |}
-        | Star vs l r =>
-          match hash _ l, hash _ r with
-            | existT vl hl , existT vr hr =>
-              @existT _ _ (vl ++ vr)
-                (join_SHeap 
-                  match  (app_nil_r vr) in _ = t return SHeap (vl ++ t) vs with
-                    | refl_equal => 
-                      @liftSHeapU vl vr nil vs 
-                        match eq_sym (app_nil_r vl) in _ = t return SHeap t vs with
-                          | refl_equal => hl
-                        end
-                  end
-                  (@liftSHeapU nil vl vr vs hr))
-          end
-        | Exists vs t b =>
-          match hash _ b with
-            | existT v b =>
-              @existT _ (fun x : list (tvar types) => SHeap x vs) (v ++ t :: nil) _
-          end
-(*
-        | Func v f a =>
-          @existT _ _ nil
-            {| funcs := dmap_insert (fun x y => Some (@finCmp _ sfuncs x y)) f (a :: nil) dmap_empty
-             ; pures := nil
-             ; other := nil
-             |}
-        | Const vars c => 
-          @existT _ _ nil
-            {| funcs := dmap_empty
-             ; pures := nil
-             ; other := c :: nil
-             |}
-             *)
-        | _ => @existT _ _ nil {| funcs := dmap_empty
-                                ; pures := nil
-                                ; other := nil
-                                |}
-      end).
-
-*)
-
-(*
-    Fixpoint hash_left' uvars vars ext (s : sexpr fs sfuncs uvars vars) {struct s} :
-      { es : variables types & 
-        { h : SHeap uvars (ext ++ es ++ vars) | forall A B C cs, heq A B C cs (existsEach _ es (denote h)) (liftSExpr nil ext _ s) } }.
-    refine (
-      match s in sexpr _ _ _ vars return { es : variables types & SHeap uvars (ext ++ es ++ vars) } with
-        | Emp _ => @existT _ _ nil (SHeap_empty _ _)
-        | Inj _ p => @existT _ _ nil 
-          {| funcs := dmap_empty
-           ; pures := @liftPures uvars nil ext _ (p :: nil) 
-           ; other := nil
-           |}
-        | Star vs l r => _
-        | _ => _
-      end).
-    refine (match @hash_left' uvars vs ext l with
-              | existT vs' l' =>
-                match hash_left' uvars vs (ext ++ vs') r with
-                  | existT vs'' r' =>
-                    @existT _ _ (vs' ++ vs'') _
-                end
-            end).
-    Check liftFunctions.
-    rewrite list_app_assoc. rewrite <- list_app_assoc. 
-    eapply join_SHeap.
-    refine (@liftSHeap uvars (ext ++ vs') vs'' vs match sym_eq (list_app_assoc ext vs' vs) in _ = t return SHeap uvars t with
-                                                 | refl_equal => l'
-                                               end).
-    apply r'.
-    clear hash_left'; admit.
-    clear hash_left'; admit.
-    clear hash_left'; admit.
-    Defined.
-
-    Fixpoint hlist_app T F (ll lr : list T) : hlist F ll -> hlist F lr -> hlist F (ll ++ lr) :=
-      match ll with
-        | nil => fun _ x => x
-        | _ :: _ => fun l r => HCons (hlist_hd l) (hlist_app (hlist_tl l) r)
-      end.
-
-    Lemma existsEach_p : forall z z' z'' (A : hlist _ z) (B : hlist _ z') (C : hlist _ z'') cs vs l r , 
-      (forall k : hlist _ vs, himp A B (hlist_app k C) cs l (liftSExpr nil vs _ r)) -> 
-      himp A B C cs (existsEach vs _ l) r.
-    Proof.
-(*
-      induction vs. simpl. split. unfold himp, ST.heq in *. intros. specialize (H HNil). auto.
-        eauto.
-
-      intros; simpl in *. split; intros.
-      
-      exists HNil. auto.
-      intros. simpl in *. destruct (IHvs (Exists _ l) (Exists _ r)). clear IHvs. unfold heq in *.
-      split; intros. simpl in *. destruct H0. 2: apply H. Focus 2. destruct H1. exists (hlist_tl x0). admit.
-      destruct H1.
-
-
-etransitivity. 2: eapply H. reflexivity. destruct H1. exists (hlist_tl x). simpl in *.
-        
-      
-      
-      .
-      destruct H. unfold heq, ST.heq in *; tauto.
-    unfold heq.
-*)
-    Admitted.
-
-    Lemma existsEach_c : forall z z' z'' (A : hlist _ z) (B : hlist _ z') (C : hlist _ z'') cs vs l r , 
-      (exists k : hlist _ vs, himp A B (hlist_app k C) cs (liftSExpr nil vs _ l) r) -> 
-      himp A B C cs l (existsEach vs _ r).
-    Proof.
-(*
-      induction vs. simpl. split. unfold himp, ST.heq in *. intros. specialize (H HNil). auto.
-        eauto.
-
-      intros; simpl in *. split; intros.
-      
-      exists HNil. auto.
-      intros. simpl in *. destruct (IHvs (Exists _ l) (Exists _ r)). clear IHvs. unfold heq in *.
-      split; intros. simpl in *. destruct H0. 2: apply H. Focus 2. destruct H1. exists (hlist_tl x0). admit.
-      destruct H1.
-
-
-etransitivity. 2: eapply H. reflexivity. destruct H1. exists (hlist_tl x). simpl in *.
-        
-      
-      
-      .
-      destruct H. unfold heq, ST.heq in *; tauto.
-    unfold heq.
-*)
-    Admitted.
-
-    Lemma liftSExpr_existsEach_c : forall cs l E a A B C P Q,
-      himp A B C cs P (existsEach E a (liftSExpr l E a Q)) ->
-      himp A B C cs P (liftSExpr l E a (existsEach E a Q)).
-
-
-    Ltac cancel_all :=
-      let s :=
-        (   reflexivity 
-         || simple apply ST.himp_star_emp_c
-         || simple apply ST.himp_star_emp_p
-         || simple apply ST.himp_star_cancel
-(*         || simple apply ST.heq_star_cancel
-         || simple apply ST.heq_star_emp
-         || (match goal with
-               | [ |- ST.heq _ _ _ ] => symmetry; simple apply ST.heq_star_emp; symmetry
-             end)
-*)
-        )
-      in
-      let perm :=
-        try ((eapply ST.himp_star_comm_p; repeat simple apply ST.himp_star_assoc_p)
-(*             (eapply ST.heq_star_comm; symmetry; repeat simple apply ST.heq_star_assoc; symmetry) *)); 
-        try do 10 (s || 
-          match goal with
-            | [ |- ST.heq _ _ _ _ _ ] =>
-              symmetry; simple apply ST.heq_star_comm; symmetry; repeat simple apply ST.heq_star_assoc
-            | [ |- ST.himp _ _ _ _ _ ] =>
-              repeat (simple apply ST.himp_star_assoc_c)
-          end)
-      in
-      do 10 perm.
-
-
-    Theorem denote_hash_left' : forall a E (s : sexpr fs sfuncs _ (E ++ a)) G cs, 
-      heq HNil HNil G cs (@existsEach nil E _ s)
-        (@existsEach _ E _ (@existsEach nil (projT1 (hash_left' nil s)) (E ++ a) (denote (projT2 (hash_left' nil s))))).
-    Proof.
-      clear. Require Import Program. dependent induction s; simpl; intros; unfold denote; simpl.
-      Focus.
-      split; eapply existsEach_p; intros; simpl. eapply existsEach_c.
-      split; eapply existsEachPf; unfold himp; intros; simpl. simple apply ST.himp_star_emp_c. apply ST.himp_star_assoc_c. 
-        apply ST.himp_star_comm_c. apply ST.himp_star_assoc_c. do 2 apply ST.himp_star_emp_c. 
-
-        
-
-        generalize (existsEachPf). unfold himp. intros. eapply H. intros. simpl. cancel_all.
-        
-
-      xxx.
-      admit. (** SIMPLE **)
-      admit. (** SIMPLE **)
-      
-
-      simpl.
-
-generalize (@nil. induction s; simpl; intros; unfold denote; simpl. 
-          admit. (** TRIVIAL **)
-          admit. (** TRIVIAL **)
-          unfold heq. simpl.
-
-          
-          admit. (** CHECK **)
-          unfold heq. simpl. admit.
-          admit. (** TRIVIAL **)
-          admit. (** TRIVIAL **)
-        
-        
-      Admitted.
-*)
